<?xml version="1.0"?>
<rdf:RDF xmlns="https://www.AHDB/connected#"
     xml:base="https://www.AHDB/connected"
     xmlns:dc="http://purl.org/dc/elements/1.1/"
     xmlns:mco="http://sbmi.uth.edu/ontology/mco#"
     xmlns:ont="http://www.co-ode.org/ontologies/ont.owl#"
     xmlns:owl="http://www.w3.org/2002/07/owl#"
     xmlns:rdf="http://www.w3.org/1999/02/22-rdf-syntax-ns#"
     xmlns:xml="http://www.w3.org/XML/1998/namespace"
     xmlns:xsd="http://www.w3.org/2001/XMLSchema#"
     xmlns:dcat="http://www.w3.org/ns/dcat#"
     xmlns:foaf="http://xmlns.com/foaf/0.1/"
     xmlns:rdfs="http://www.w3.org/2000/01/rdf-schema#"
     xmlns:skos="http://www.w3.org/2004/02/skos/core#"
     xmlns:void="http://rdfs.org/ns/void#"
     xmlns:dcterms="http://purl.org/dc/terms/"
     xmlns:oboInOwl="http://www.geneontology.org/formats/oboInOwl#">
    <owl:Ontology/>
    


    <!-- 
    ///////////////////////////////////////////////////////////////////////////////////////
    //
    // Annotation properties
    //
    ///////////////////////////////////////////////////////////////////////////////////////
     -->

    


    <!-- http://purl.org/dc/elements/1.1/creator -->

    <owl:AnnotationProperty rdf:about="http://purl.org/dc/elements/1.1/creator"/>
    


    <!-- http://purl.org/dc/elements/1.1/description -->

    <owl:AnnotationProperty rdf:about="http://purl.org/dc/elements/1.1/description"/>
    


    <!-- http://purl.org/dc/elements/1.1/title -->

    <owl:AnnotationProperty rdf:about="http://purl.org/dc/elements/1.1/title"/>
    


    <!-- http://purl.org/dc/terms/created -->

    <owl:AnnotationProperty rdf:about="http://purl.org/dc/terms/created"/>
    


    <!-- http://purl.org/dc/terms/creator -->

    <owl:AnnotationProperty rdf:about="http://purl.org/dc/terms/creator"/>
    


    <!-- http://purl.org/dc/terms/description -->

    <owl:AnnotationProperty rdf:about="http://purl.org/dc/terms/description"/>
    


    <!-- http://purl.org/dc/terms/publisher -->

    <owl:AnnotationProperty rdf:about="http://purl.org/dc/terms/publisher"/>
    


    <!-- http://purl.org/dc/terms/subject -->

    <owl:AnnotationProperty rdf:about="http://purl.org/dc/terms/subject"/>
    


    <!-- http://purl.org/dc/terms/title -->

    <owl:AnnotationProperty rdf:about="http://purl.org/dc/terms/title"/>
    


    <!-- http://rdfs.org/ns/void#dataDump -->

    <owl:AnnotationProperty rdf:about="http://rdfs.org/ns/void#dataDump"/>
    


    <!-- http://rdfs.org/ns/void#triples -->

    <owl:AnnotationProperty rdf:about="http://rdfs.org/ns/void#triples"/>
    


    <!-- http://sbmi.uth.edu/ontology/mco#contact_text -->

    <owl:AnnotationProperty rdf:about="http://sbmi.uth.edu/ontology/mco#contact_text"/>
    


    <!-- http://sbmi.uth.edu/ontology/mco#documentation -->

    <owl:AnnotationProperty rdf:about="http://sbmi.uth.edu/ontology/mco#documentation"/>
    


    <!-- http://sbmi.uth.edu/ontology/mco#name_text -->

    <owl:AnnotationProperty rdf:about="http://sbmi.uth.edu/ontology/mco#name_text"/>
    


    <!-- http://sbmi.uth.edu/ontology/mco#overview -->

    <owl:AnnotationProperty rdf:about="http://sbmi.uth.edu/ontology/mco#overview"/>
    


    <!-- http://www.geneontology.org/formats/oboInOwl#created_by -->

    <owl:AnnotationProperty rdf:about="http://www.geneontology.org/formats/oboInOwl#created_by"/>
    


    <!-- http://www.geneontology.org/formats/oboInOwl#creation_date -->

    <owl:AnnotationProperty rdf:about="http://www.geneontology.org/formats/oboInOwl#creation_date"/>
    


    <!-- http://www.w3.org/2004/02/skos/core#closeMatch -->

    <owl:AnnotationProperty rdf:about="http://www.w3.org/2004/02/skos/core#closeMatch"/>
    


    <!-- http://xmlns.com/foaf/0.1/homepage -->

    <owl:AnnotationProperty rdf:about="http://xmlns.com/foaf/0.1/homepage"/>
    


    <!-- http://xmlns.com/foaf/0.1/mbox -->

    <owl:AnnotationProperty rdf:about="http://xmlns.com/foaf/0.1/mbox"/>
    


    <!-- 
    ///////////////////////////////////////////////////////////////////////////////////////
    //
    // Object Properties
    //
    ///////////////////////////////////////////////////////////////////////////////////////
     -->

    


    <!-- http://www.co-ode.org/ontologies/ont.owl#describe -->

    <owl:ObjectProperty rdf:about="http://www.co-ode.org/ontologies/ont.owl#describe">
        <owl:inverseOf rdf:resource="http://www.co-ode.org/ontologies/ont.owl#hasCode"/>
        <rdfs:label>describe</rdfs:label>
    </owl:ObjectProperty>
    


    <!-- http://www.co-ode.org/ontologies/ont.owl#hasCode -->

    <owl:ObjectProperty rdf:about="http://www.co-ode.org/ontologies/ont.owl#hasCode">
        <dcterms:created rdf:datatype="http://www.w3.org/2001/XMLSchema#integer">1747008000</dcterms:created>
        <dcterms:creator>AlmaHealthDB</dcterms:creator>
        <dcterms:description>This property associates model input or output with its corresponding LOINC code, a standardized identifier used in the LOINC terminology to uniquely represent clinical data.</dcterms:description>
        <rdfs:comment>links an input or an output to its corresponding LOINC code</rdfs:comment>
        <rdfs:label>hasCode</rdfs:label>
    </owl:ObjectProperty>
    


    <!-- http://www.co-ode.org/ontologies/ont.owl#interfaceInput -->

    <owl:ObjectProperty rdf:about="http://www.co-ode.org/ontologies/ont.owl#interfaceInput">
        <rdfs:domain rdf:resource="https://www.AHDB/connected#InputMapping"/>
        <rdfs:range rdf:resource="https://www.AHDB/connected#Input"/>
        <dcterms:created rdf:datatype="http://www.w3.org/2001/XMLSchema#integer">1747008000</dcterms:created>
        <dcterms:creator>AlmaHealthDB</dcterms:creator>
        <dcterms:description>This property associates a concrete input parameter, as defined in the implementation of an interface, with its corresponding description.</dcterms:description>
        <rdfs:comment>links a concrete input parameter of an interface implementation to its description.</rdfs:comment>
        <rdfs:label>interfaceInput</rdfs:label>
    </owl:ObjectProperty>
    


    <!-- http://www.co-ode.org/ontologies/ont.owl#interfaceOutput -->

    <owl:ObjectProperty rdf:about="http://www.co-ode.org/ontologies/ont.owl#interfaceOutput">
        <rdfs:domain rdf:resource="https://www.AHDB/connected#OutputMapping"/>
        <rdfs:range rdf:resource="https://www.AHDB/connected#Output"/>
        <dcterms:created rdf:datatype="http://www.w3.org/2001/XMLSchema#integer">1747008000</dcterms:created>
        <dcterms:creator>AlmaHealthDB</dcterms:creator>
        <dcterms:description>This property associates a concrete output parameter, as defined in the implementation of an interface, with its corresponding description.</dcterms:description>
        <rdfs:comment>links a concrete output parameter of an interface implementation to its description.</rdfs:comment>
        <rdfs:label>interfaceOutput</rdfs:label>
    </owl:ObjectProperty>
    


    <!-- http://www.w3.org/2004/02/skos/core#broader -->

    <owl:ObjectProperty rdf:about="http://www.w3.org/2004/02/skos/core#broader"/>
    


    <!-- https://www.AHDB/connected#expects -->

    <owl:ObjectProperty rdf:about="https://www.AHDB/connected#expects">
        <rdf:type rdf:resource="http://www.w3.org/2002/07/owl#AsymmetricProperty"/>
        <rdf:type rdf:resource="http://www.w3.org/2002/07/owl#IrreflexiveProperty"/>
        <rdfs:domain rdf:resource="https://www.AHDB/connected#Interface"/>
        <rdfs:range rdf:resource="https://www.AHDB/connected#Input"/>
        <dcterms:created rdf:datatype="http://www.w3.org/2001/XMLSchema#integer">1746144000</dcterms:created>
        <dcterms:creator>AlmaHealthDB</dcterms:creator>
        <dcterms:description>This property links a model interface to Inputs that must be provided when calling the interface. It defines the expected parameters required for execution.</dcterms:description>
        <rdfs:comment>Connects a model interface to a parameter description</rdfs:comment>
        <rdfs:label>expects</rdfs:label>
    </owl:ObjectProperty>
    


    <!-- https://www.AHDB/connected#hasInterface -->

    <owl:ObjectProperty rdf:about="https://www.AHDB/connected#hasInterface">
        <rdf:type rdf:resource="http://www.w3.org/2002/07/owl#InverseFunctionalProperty"/>
        <rdf:type rdf:resource="http://www.w3.org/2002/07/owl#AsymmetricProperty"/>
        <rdf:type rdf:resource="http://www.w3.org/2002/07/owl#IrreflexiveProperty"/>
        <rdfs:domain rdf:resource="https://www.AHDB/connected#Model"/>
        <rdfs:range rdf:resource="https://www.AHDB/connected#Interface"/>
        <dcterms:created rdf:datatype="http://www.w3.org/2001/XMLSchema#integer">1746144000</dcterms:created>
        <dcterms:creator>AlmaHealthDB</dcterms:creator>
        <dcterms:description>This property links a model to its specific exposing interface</dcterms:description>
        <rdfs:comment>links a Model to its exposing Inteface</rdfs:comment>
        <rdfs:label>hasInterface</rdfs:label>
    </owl:ObjectProperty>
    


    <!-- https://www.AHDB/connected#hasMaintainer -->

    <owl:ObjectProperty rdf:about="https://www.AHDB/connected#hasMaintainer">
        <rdf:type rdf:resource="http://www.w3.org/2002/07/owl#AsymmetricProperty"/>
        <rdf:type rdf:resource="http://www.w3.org/2002/07/owl#IrreflexiveProperty"/>
        <rdfs:domain rdf:resource="https://www.AHDB/connected#Model"/>
        <rdfs:range rdf:resource="https://www.AHDB/connected#Mantainer"/>
        <dcterms:created rdf:datatype="http://www.w3.org/2001/XMLSchema#integer">1746144000</dcterms:created>
        <dcterms:creator>AlmaHealthDB</dcterms:creator>
        <dcterms:description>This property links a model to its maintaner</dcterms:description>
        <rdfs:comment>links a Model to its maintainer</rdfs:comment>
        <rdfs:label>hasMaintainer</rdfs:label>
    </owl:ObjectProperty>
    


    <!-- https://www.AHDB/connected#implementation -->

    <owl:ObjectProperty rdf:about="https://www.AHDB/connected#implementation">
        <rdf:type rdf:resource="http://www.w3.org/2002/07/owl#FunctionalProperty"/>
        <rdf:type rdf:resource="http://www.w3.org/2002/07/owl#InverseFunctionalProperty"/>
        <rdf:type rdf:resource="http://www.w3.org/2002/07/owl#AsymmetricProperty"/>
        <rdf:type rdf:resource="http://www.w3.org/2002/07/owl#IrreflexiveProperty"/>
        <rdfs:domain rdf:resource="https://www.AHDB/connected#Mapping"/>
        <rdfs:range rdf:resource="https://www.AHDB/connected#Implementation"/>
        <dcterms:created rdf:datatype="http://www.w3.org/2001/XMLSchema#integer">1746144000</dcterms:created>
        <dcterms:creator>AlmaHealthDB</dcterms:creator>
        <dcterms:description>This property links an implementation to a mapping, which serves as the binding point between the formal interface definition and its concrete realization.</dcterms:description>
        <rdfs:comment>specifies a concrete implementation within a mapping</rdfs:comment>
        <rdfs:label>implementation</rdfs:label>
    </owl:ObjectProperty>
    


    <!-- https://www.AHDB/connected#inputMapping -->

    <owl:ObjectProperty rdf:about="https://www.AHDB/connected#inputMapping">
        <rdf:type rdf:resource="http://www.w3.org/2002/07/owl#AsymmetricProperty"/>
        <rdf:type rdf:resource="http://www.w3.org/2002/07/owl#IrreflexiveProperty"/>
        <rdfs:domain rdf:resource="https://www.AHDB/connected#Mapping"/>
        <rdfs:range rdf:resource="https://www.AHDB/connected#InputMapping"/>
        <dcterms:created rdf:datatype="http://www.w3.org/2001/XMLSchema#integer">1746144000</dcterms:created>
        <dcterms:creator>AlmaHealthDB</dcterms:creator>
        <dcterms:description>This property connects an abstract input to a mapping, which serves as the binding point between its formal interface definition and its concrete realization.</dcterms:description>
        <rdfs:comment>links a mapping  to an inputMapping</rdfs:comment>
        <rdfs:label>inputMapping</rdfs:label>
    </owl:ObjectProperty>
    


    <!-- https://www.AHDB/connected#interface -->

    <owl:ObjectProperty rdf:about="https://www.AHDB/connected#interface">
        <rdf:type rdf:resource="http://www.w3.org/2002/07/owl#FunctionalProperty"/>
        <rdf:type rdf:resource="http://www.w3.org/2002/07/owl#InverseFunctionalProperty"/>
        <rdf:type rdf:resource="http://www.w3.org/2002/07/owl#AsymmetricProperty"/>
        <rdf:type rdf:resource="http://www.w3.org/2002/07/owl#IrreflexiveProperty"/>
        <rdfs:domain rdf:resource="https://www.AHDB/connected#Mapping"/>
        <rdfs:range rdf:resource="https://www.AHDB/connected#Interface"/>
        <dcterms:created rdf:datatype="http://www.w3.org/2001/XMLSchema#integer">1746144000</dcterms:created>
        <dcterms:creator>AlmaHealthDB</dcterms:creator>
        <dcterms:description>This property links a model interface to a mapping, which serves as the binding point between its formal definition and its concrete realization.</dcterms:description>
        <rdfs:comment>links a concrete mapping to a model interface</rdfs:comment>
        <rdfs:label>interface</rdfs:label>
    </owl:ObjectProperty>
    


    <!-- https://www.AHDB/connected#outputMapping -->

    <owl:ObjectProperty rdf:about="https://www.AHDB/connected#outputMapping">
        <rdf:type rdf:resource="http://www.w3.org/2002/07/owl#AsymmetricProperty"/>
        <rdf:type rdf:resource="http://www.w3.org/2002/07/owl#IrreflexiveProperty"/>
        <rdfs:domain rdf:resource="https://www.AHDB/connected#Mapping"/>
        <rdfs:range rdf:resource="https://www.AHDB/connected#OutputMapping"/>
        <dcterms:created rdf:datatype="http://www.w3.org/2001/XMLSchema#integer">1746144000</dcterms:created>
        <dcterms:creator>AlmaHealthDB</dcterms:creator>
        <dcterms:description>This property connects an abstract output to a mapping, which serves as the binding point between its formal interface definition and its concrete realization.</dcterms:description>
        <rdfs:comment>links a mapping  to an outputMapping</rdfs:comment>
        <rdfs:label>outputMapping</rdfs:label>
    </owl:ObjectProperty>
    


    <!-- https://www.AHDB/connected#returns -->

    <owl:ObjectProperty rdf:about="https://www.AHDB/connected#returns">
        <rdf:type rdf:resource="http://www.w3.org/2002/07/owl#AsymmetricProperty"/>
        <rdf:type rdf:resource="http://www.w3.org/2002/07/owl#IrreflexiveProperty"/>
        <rdfs:domain rdf:resource="https://www.AHDB/connected#Interface"/>
        <rdfs:range rdf:resource="https://www.AHDB/connected#Output"/>
        <dcterms:created rdf:datatype="http://www.w3.org/2001/XMLSchema#integer">1746144000</dcterms:created>
        <dcterms:creator>AlmaHealthDB</dcterms:creator>
        <dcterms:description>This property links a model interface to Outputs that must be provided when calling the interface. It defines the expected parameters required for execution.</dcterms:description>
        <rdfs:comment>Connects a model interface to an output description</rdfs:comment>
        <rdfs:label>returns</rdfs:label>
    </owl:ObjectProperty>
    


    <!-- 
    ///////////////////////////////////////////////////////////////////////////////////////
    //
    // Data properties
    //
    ///////////////////////////////////////////////////////////////////////////////////////
     -->

    


    <!-- http://xmlns.com/foaf/0.1/familyName -->

    <owl:DatatypeProperty rdf:about="http://xmlns.com/foaf/0.1/familyName"/>
    


    <!-- http://xmlns.com/foaf/0.1/givenName -->

    <owl:DatatypeProperty rdf:about="http://xmlns.com/foaf/0.1/givenName"/>
    


    <!-- http://xmlns.com/foaf/0.1/name -->

    <owl:DatatypeProperty rdf:about="http://xmlns.com/foaf/0.1/name"/>
    


    <!-- https://www.AHDB/connected#contentType -->

    <owl:DatatypeProperty rdf:about="https://www.AHDB/connected#contentType">
        <rdfs:domain rdf:resource="https://www.AHDB/connected#WebAPI"/>
        <rdfs:range rdf:resource="http://www.w3.org/2001/XMLSchema#string"/>
        <dcterms:created rdf:datatype="http://www.w3.org/2001/XMLSchema#integer">1746144000</dcterms:created>
        <dcterms:creator>AlmaHealthDB</dcterms:creator>
        <dcterms:description>This property indicates the expected content type (e.g., &apos;application/json&apos;, &apos;text/csv&apos;) for data sent to a WebAPI. It allows clients to understand how to format their requests properly.</dcterms:description>
        <rdfs:comment>defines the Content-type of the resources expected by the WebAPI</rdfs:comment>
        <rdfs:label>contentType</rdfs:label>
    </owl:DatatypeProperty>
    


    <!-- https://www.AHDB/connected#entrypoint -->

    <owl:DatatypeProperty rdf:about="https://www.AHDB/connected#entrypoint">
        <rdfs:domain rdf:resource="https://www.AHDB/connected#WebAPI"/>
        <rdfs:range rdf:resource="http://www.w3.org/2001/XMLSchema#anyURI"/>
        <dcterms:created rdf:datatype="http://www.w3.org/2001/XMLSchema#integer">1746144000</dcterms:created>
        <dcterms:creator>AlmaHealthDB</dcterms:creator>
        <dcterms:description>This property defines the actual endpoint (typically an HTTP or HTTPS URI) through which the WebAPI can be invoked by clients.</dcterms:description>
        <rdfs:comment>defines the entrypoint to contact the WebAPI</rdfs:comment>
        <rdfs:label>entrypoint</rdfs:label>
    </owl:DatatypeProperty>
    


    <!-- https://www.AHDB/connected#method -->

    <owl:DatatypeProperty rdf:about="https://www.AHDB/connected#method">
        <rdfs:domain rdf:resource="https://www.AHDB/connected#WebAPI"/>
        <rdfs:range rdf:resource="http://www.w3.org/2001/XMLSchema#anyURI"/>
        <dcterms:created rdf:datatype="http://www.w3.org/2001/XMLSchema#integer">1746144000</dcterms:created>
        <dcterms:creator>AlmaHealthDB</dcterms:creator>
        <dcterms:description>This property indicates which HTTP method (e.g., &apos;GET&apos;, &apos;POST&apos;) must be used when invoking the WebAPI endpoint.</dcterms:description>
        <rdfs:comment>defines the method exposed by the WebAPI</rdfs:comment>
        <rdfs:label>method</rdfs:label>
    </owl:DatatypeProperty>
    


    <!-- https://www.AHDB/connected#position -->

    <owl:DatatypeProperty rdf:about="https://www.AHDB/connected#position">
        <rdfs:domain rdf:resource="https://www.AHDB/connected#PositionInputMapping"/>
        <rdfs:range rdf:resource="http://www.w3.org/2001/XMLSchema#integer"/>
        <dcterms:created rdf:datatype="http://www.w3.org/2001/XMLSchema#integer">1746144000</dcterms:created>
        <dcterms:creator>AlmaHealthDB</dcterms:creator>
        <dcterms:description>This property specifies the position of an input parameter passed to the concrete implementation of an interface.</dcterms:description>
        <rdfs:comment>defines the position of the input</rdfs:comment>
        <rdfs:label>position</rdfs:label>
    </owl:DatatypeProperty>
    


    <!-- https://www.AHDB/connected#property -->

    <owl:DatatypeProperty rdf:about="https://www.AHDB/connected#property">
        <rdfs:domain rdf:resource="https://www.AHDB/connected#PropertyInputMapping"/>
        <rdfs:range rdf:resource="http://www.w3.org/2001/XMLSchema#integer"/>
        <dcterms:created rdf:datatype="http://www.w3.org/2001/XMLSchema#integer">1746144000</dcterms:created>
        <dcterms:creator>AlmaHealthDB</dcterms:creator>
        <dcterms:description>This property specifies the name of the input parameter as it is passed to the concrete implementation of an interface.</dcterms:description>
        <rdfs:comment>defines the mapped property name</rdfs:comment>
        <rdfs:label>property</rdfs:label>
    </owl:DatatypeProperty>
    


    <!-- https://www.AHDB/connected#required -->

    <owl:DatatypeProperty rdf:about="https://www.AHDB/connected#required">
        <rdfs:domain rdf:resource="https://www.AHDB/connected#Input"/>
        <rdfs:range rdf:resource="http://www.w3.org/2001/XMLSchema#boolean"/>
        <dcterms:created rdf:datatype="http://www.w3.org/2001/XMLSchema#integer">1746144000</dcterms:created>
        <dcterms:creator>AlmaHealthDB</dcterms:creator>
        <dcterms:description>This property specifies whether the input is required (true) or optional (false) when invoking the interface.</dcterms:description>
        <rdfs:comment>specifies if the input is required or not</rdfs:comment>
        <rdfs:label>required</rdfs:label>
    </owl:DatatypeProperty>
    


    <!-- https://www.AHDB/connected#template -->

    <owl:DatatypeProperty rdf:about="https://www.AHDB/connected#template">
        <rdfs:domain rdf:resource="https://www.AHDB/connected#WebAPI"/>
        <rdfs:range rdf:resource="http://www.w3.org/2001/XMLSchema#string"/>
        <dcterms:created rdf:datatype="http://www.w3.org/2001/XMLSchema#integer">1746144000</dcterms:created>
        <dcterms:creator>AlmaHealthDB</dcterms:creator>
        <dcterms:description>This property defines a string or object that outlines the expected keys and their associated value types or formats. It is intended to guide data consumers or processors in understanding the structure and requirements of a given data template</dcterms:description>
        <rdfs:comment>defines string or object that outlines the expected keys and their value types or formats</rdfs:comment>
        <rdfs:label>template</rdfs:label>
    </owl:DatatypeProperty>
    


    <!-- https://www.AHDB/connected#type -->

    <owl:DatatypeProperty rdf:about="https://www.AHDB/connected#type">
        <rdfs:domain>
            <owl:Class>
                <owl:unionOf rdf:parseType="Collection">
                    <rdf:Description rdf:about="https://www.AHDB/connected#Input"/>
                    <rdf:Description rdf:about="https://www.AHDB/connected#Output"/>
                </owl:unionOf>
            </owl:Class>
        </rdfs:domain>
        <dcterms:created rdf:datatype="http://www.w3.org/2001/XMLSchema#integer">1746144000</dcterms:created>
        <dcterms:creator>AlmaHealthDB</dcterms:creator>
        <dcterms:description>This property defines the data type (e.g., string, integer...) expected for an input or output.</dcterms:description>
        <rdfs:comment>defines the Input&apos;s or the output&apos;s type</rdfs:comment>
        <rdfs:label>type</rdfs:label>
    </owl:DatatypeProperty>
    


    <!-- 
    ///////////////////////////////////////////////////////////////////////////////////////
    //
    // Classes
    //
    ///////////////////////////////////////////////////////////////////////////////////////
     -->

    


    <!-- http://www.w3.org/2000/10/swap/pim/contact#Person -->

    <owl:Class rdf:about="http://www.w3.org/2000/10/swap/pim/contact#Person"/>
    


    <!-- https://www.AHDB/connected#Implementation -->

    <owl:Class rdf:about="https://www.AHDB/connected#Implementation">
        <dcterms:created rdf:datatype="http://www.w3.org/2001/XMLSchema#integer">1746144000</dcterms:created>
        <dcterms:creator>AlmaHealthDB</dcterms:creator>
        <dcterms:description>A class that corresponds to operational components or services that fulfill the defined behavior of a model.</dcterms:description>
        <rdfs:comment>An Implementation defines the internal workings of one or more Interface</rdfs:comment>
        <rdfs:label>Implementation</rdfs:label>
    </owl:Class>
    


    <!-- https://www.AHDB/connected#Input -->

    <owl:Class rdf:about="https://www.AHDB/connected#Input">
        <owl:disjointWith rdf:resource="https://www.AHDB/connected#Output"/>
        <dcterms:created rdf:datatype="http://www.w3.org/2001/XMLSchema#integer">1746144000</dcterms:created>
        <dcterms:creator>AlmaHealthDB</dcterms:creator>
        <dcterms:description>A class that describes the formal structure of an input of an interface.</dcterms:description>
        <rdfs:comment>An Input is the description of the input value of an Interface.</rdfs:comment>
        <rdfs:label>Input</rdfs:label>
    </owl:Class>
    


    <!-- https://www.AHDB/connected#InputMapping -->

    <owl:Class rdf:about="https://www.AHDB/connected#InputMapping">
        <owl:disjointWith rdf:resource="https://www.AHDB/connected#OutputMapping"/>
        <dcterms:created rdf:datatype="http://www.w3.org/2001/XMLSchema#integer">1746144000</dcterms:created>
        <dcterms:creator>AlmaHealthDB</dcterms:creator>
        <dcterms:description>A class that defines the practical implementation of an input for a specific interface, mapping actual data to the formal specification.</dcterms:description>
        <rdfs:comment>An input mapping clearly defines how an abstract parameter corresponds to a method&apos;s argument, either by position (e.g., the third argument) or by property name (e.g., in Web APIs).</rdfs:comment>
        <rdfs:label>InputMapping</rdfs:label>
    </owl:Class>
    


    <!-- https://www.AHDB/connected#Interface -->

    <owl:Class rdf:about="https://www.AHDB/connected#Interface">
        <dcterms:created rdf:datatype="http://www.w3.org/2001/XMLSchema#integer">1746144000</dcterms:created>
        <dcterms:creator>AlmaHealthDB</dcterms:creator>
        <dcterms:description>A class that defines a formal interface for interacting with the model</dcterms:description>
        <rdfs:comment>An Interface is a process that performs a specific task by associating one or more Parameters to an Output</rdfs:comment>
        <rdfs:label>Interface</rdfs:label>
    </owl:Class>
    


    <!-- https://www.AHDB/connected#Mantainer -->

    <owl:Class rdf:about="https://www.AHDB/connected#Mantainer">
        <dcterms:created rdf:datatype="http://www.w3.org/2001/XMLSchema#integer">1746144000</dcterms:created>
        <dcterms:creator>AlmaHealthDB</dcterms:creator>
        <dcterms:description>A class representing an individual or entity responsible for the maintenance, and updating of a machine learning model.</dcterms:description>
        <rdfs:comment>Maintainer is individual or organization responsible for the ongoing management, validation, and updates of the model</rdfs:comment>
        <rdfs:label>Mantainer</rdfs:label>
    </owl:Class>
    


    <!-- https://www.AHDB/connected#Mapping -->

    <owl:Class rdf:about="https://www.AHDB/connected#Mapping">
        <dcterms:created rdf:datatype="http://www.w3.org/2001/XMLSchema#integer">1746144000</dcterms:created>
        <dcterms:creator>AlmaHealthDB</dcterms:creator>
        <dcterms:description>A class representing the binding between an abstract interface and a concrete implementation.</dcterms:description>
        <rdfs:comment>A Mapping links (abstract) Interface and (concrete) Implementation</rdfs:comment>
        <rdfs:label>Mapping</rdfs:label>
    </owl:Class>
    


    <!-- https://www.AHDB/connected#Model -->

    <owl:Class rdf:about="https://www.AHDB/connected#Model">
        <dcterms:created rdf:datatype="http://www.w3.org/2001/XMLSchema#integer">1746144000</dcterms:created>
        <dcterms:creator>AlmaHealthDB</dcterms:creator>
        <dcterms:description>A class that rapresent a machine learning/computational/predictive model</dcterms:description>
        <rdfs:comment>A model is a formal abstraction or conceptualization that encapsulates the behavior, purpose, and intended usage of a machine learning model, independent of its specific implementation details</rdfs:comment>
        <rdfs:label>Model</rdfs:label>
    </owl:Class>
    


    <!-- https://www.AHDB/connected#Output -->

    <owl:Class rdf:about="https://www.AHDB/connected#Output">
        <dcterms:created rdf:datatype="http://www.w3.org/2001/XMLSchema#integer">1746144000</dcterms:created>
        <dcterms:creator>AlmaHealthDB</dcterms:creator>
        <dcterms:description>A class that describes the formal structure of an output of an interface.</dcterms:description>
        <rdfs:comment>An Output is the description of the output value of an Interface.</rdfs:comment>
        <rdfs:label>Output</rdfs:label>
    </owl:Class>
    


    <!-- https://www.AHDB/connected#OutputMapping -->

    <owl:Class rdf:about="https://www.AHDB/connected#OutputMapping">
        <dcterms:created rdf:datatype="http://www.w3.org/2001/XMLSchema#integer">1746144000</dcterms:created>
        <dcterms:creator>AlmaHealthDB</dcterms:creator>
        <dcterms:description>A class that defines the practical implementation of an output for a specific interface, mapping actual data to the formal specification.</dcterms:description>
        <rdfs:comment>An output mapping links the return value of the method to an output</rdfs:comment>
        <rdfs:label>OutputMapping</rdfs:label>
    </owl:Class>
    


    <!-- https://www.AHDB/connected#PositionInputMapping -->

    <owl:Class rdf:about="https://www.AHDB/connected#PositionInputMapping">
        <rdfs:subClassOf rdf:resource="https://www.AHDB/connected#InputMapping"/>
        <owl:disjointWith rdf:resource="https://www.AHDB/connected#PropertyInputMapping"/>
        <dcterms:created rdf:datatype="http://www.w3.org/2001/XMLSchema#integer">1746144000</dcterms:created>
        <dcterms:creator>AlmaHealthDB</dcterms:creator>
        <dcterms:description>A class that represents an input mapping where the input is passed to the interface of a model based on its positional index in the parameter list.</dcterms:description>
        <rdfs:comment>A position parameter mapping uses a position to map a parameter of an implementation to a parameter</rdfs:comment>
        <rdfs:label>PositionInputMapping</rdfs:label>
    </owl:Class>
    


    <!-- https://www.AHDB/connected#PropertyInputMapping -->

    <owl:Class rdf:about="https://www.AHDB/connected#PropertyInputMapping">
        <rdfs:subClassOf rdf:resource="https://www.AHDB/connected#InputMapping"/>
        <dcterms:created rdf:datatype="http://www.w3.org/2001/XMLSchema#integer">1746144000</dcterms:created>
        <dcterms:creator>AlmaHealthDB</dcterms:creator>
        <dcterms:description>A class that represents an input mapping where the input is passed to the interface of a model based on its name.</dcterms:description>
        <rdfs:comment>A property parameter mapping uses a property string to map a parameter of an implementation to a parameter</rdfs:comment>
        <rdfs:label>PropertyInputMapping</rdfs:label>
    </owl:Class>
    


    <!-- https://www.AHDB/connected#WebAPI -->

    <owl:Class rdf:about="https://www.AHDB/connected#WebAPI">
        <rdfs:subClassOf rdf:resource="https://www.AHDB/connected#Implementation"/>
        <dc:creator>AlmaHealthDB</dc:creator>
        <dc:description>A class that represents the implementation of a model&apos;s behavior as a Web API, exposing its operations through standardized HTTP interface</dc:description>
        <dcterms:created rdf:datatype="http://www.w3.org/2001/XMLSchema#integer">1746144000</dcterms:created>
        <rdfs:comment>an implementation of an interface as a Web API</rdfs:comment>
        <rdfs:label>WebAPI</rdfs:label>
    </owl:Class>
    


    <!-- 
    ///////////////////////////////////////////////////////////////////////////////////////
    //
    // Individuals
    //
    ///////////////////////////////////////////////////////////////////////////////////////
     -->

    


    <!-- http://loinc.org/30525-0 -->

    <owl:NamedIndividual rdf:about="http://loinc.org/30525-0"/>
    


    <!-- http://loinc.org/45643-4 -->

    <owl:NamedIndividual rdf:about="http://loinc.org/45643-4"/>
    


    <!-- http://snomed.info/sct/866240007 -->

    <owl:NamedIndividual rdf:about="http://snomed.info/sct/866240007"/>
    


    <!-- http://www.co-ode.org/ontologies/ont.owl#age -->

    <owl:NamedIndividual rdf:about="http://www.co-ode.org/ontologies/ont.owl#age">
        <rdf:type rdf:resource="https://www.AHDB/connected#Input"/>
        <ont:hasCode rdf:resource="http://loinc.org/30525-0"/>
        <required rdf:datatype="http://www.w3.org/2001/XMLSchema#boolean">true</required>
        <type>xsd:int</type>
    </owl:NamedIndividual>
    


    <!-- http://www.co-ode.org/ontologies/ont.owl#ageMapping -->

    <owl:NamedIndividual rdf:about="http://www.co-ode.org/ontologies/ont.owl#ageMapping">
        <rdf:type rdf:resource="https://www.AHDB/connected#PositionInputMapping"/>
        <ont:interfaceInput rdf:resource="http://www.co-ode.org/ontologies/ont.owl#age"/>
        <position rdf:datatype="http://www.w3.org/2001/XMLSchema#integer">0</position>
    </owl:NamedIndividual>
    


    <!-- http://www.co-ode.org/ontologies/ont.owl#avg_glucose -->

    <owl:NamedIndividual rdf:about="http://www.co-ode.org/ontologies/ont.owl#avg_glucose">
        <rdf:type rdf:resource="https://www.AHDB/connected#Input"/>
        <ont:hasCode rdf:resource="https://loinc.org/15074-8"/>
        <required rdf:datatype="http://www.w3.org/2001/XMLSchema#boolean">true</required>
        <type>xsd:double</type>
    </owl:NamedIndividual>
    


    <!-- http://www.co-ode.org/ontologies/ont.owl#avg_glucoseMapping -->

    <owl:NamedIndividual rdf:about="http://www.co-ode.org/ontologies/ont.owl#avg_glucoseMapping">
        <rdf:type rdf:resource="https://www.AHDB/connected#PositionInputMapping"/>
        <ont:interfaceInput rdf:resource="http://www.co-ode.org/ontologies/ont.owl#avg_glucose"/>
        <position rdf:datatype="http://www.w3.org/2001/XMLSchema#integer">2</position>
    </owl:NamedIndividual>
    


    <!-- http://www.co-ode.org/ontologies/ont.owl#heart_disease -->

    <owl:NamedIndividual rdf:about="http://www.co-ode.org/ontologies/ont.owl#heart_disease">
        <rdf:type rdf:resource="https://www.AHDB/connected#Input"/>
        <ont:hasCode rdf:resource="https://loinc.org/LA32903-9"/>
        <required rdf:datatype="http://www.w3.org/2001/XMLSchema#boolean">true</required>
        <type>xsd:boolean</type>
    </owl:NamedIndividual>
    


    <!-- http://www.co-ode.org/ontologies/ont.owl#heart_diseaseMapping -->

    <owl:NamedIndividual rdf:about="http://www.co-ode.org/ontologies/ont.owl#heart_diseaseMapping">
        <rdf:type rdf:resource="https://www.AHDB/connected#PositionInputMapping"/>
        <ont:interfaceInput rdf:resource="http://www.co-ode.org/ontologies/ont.owl#heart_disease"/>
        <position rdf:datatype="http://www.w3.org/2001/XMLSchema#integer">1</position>
    </owl:NamedIndividual>
    


    <!-- http://www.co-ode.org/ontologies/ont.owl#hypertension -->

    <owl:NamedIndividual rdf:about="http://www.co-ode.org/ontologies/ont.owl#hypertension">
        <rdf:type rdf:resource="https://www.AHDB/connected#Input"/>
        <ont:hasCode rdf:resource="http://loinc.org/45643-4"/>
        <required rdf:datatype="http://www.w3.org/2001/XMLSchema#boolean">true</required>
        <type>xsd:boolean</type>
    </owl:NamedIndividual>
    


    <!-- http://www.co-ode.org/ontologies/ont.owl#hypertensionMapping -->

    <owl:NamedIndividual rdf:about="http://www.co-ode.org/ontologies/ont.owl#hypertensionMapping">
        <rdf:type rdf:resource="https://www.AHDB/connected#PositionInputMapping"/>
        <ont:interfaceInput rdf:resource="http://www.co-ode.org/ontologies/ont.owl#hypertension"/>
        <position rdf:datatype="http://www.w3.org/2001/XMLSchema#integer">3</position>
    </owl:NamedIndividual>
    


    <!-- http://www.co-ode.org/ontologies/ont.owl#maintainer -->

    <owl:NamedIndividual rdf:about="http://www.co-ode.org/ontologies/ont.owl#maintainer">
        <rdf:type rdf:resource="https://www.AHDB/connected#Mantainer"/>
        <owl:sameAs rdf:resource="http://www.co-ode.org/ontologies/ont.owl#user"/>
    </owl:NamedIndividual>
    


    <!-- http://www.co-ode.org/ontologies/ont.owl#user -->

    <rdf:Description rdf:about="http://www.co-ode.org/ontologies/ont.owl#user"/>
    


    <!-- http://www.co-ode.org/ontologies/ont.owl#outMapping -->

    <owl:NamedIndividual rdf:about="http://www.co-ode.org/ontologies/ont.owl#outMapping">
        <rdf:type rdf:resource="https://www.AHDB/connected#OutputMapping"/>
        <ont:interfaceOutput rdf:resource="http://www.co-ode.org/ontologies/ont.owl#output"/>
    </owl:NamedIndividual>
    


    <!-- http://www.co-ode.org/ontologies/ont.owl#output -->

    <owl:NamedIndividual rdf:about="http://www.co-ode.org/ontologies/ont.owl#output">
        <rdf:type rdf:resource="https://www.AHDB/connected#Output"/>
        <ont:hasCode rdf:resource="http://snomed.info/sct/866240007"/>
        <type>xsd:double</type>
    </owl:NamedIndividual>
    


    <!-- http://www.co-ode.org/ontologies/ont.owl#strokeMapping -->

    <owl:NamedIndividual rdf:about="http://www.co-ode.org/ontologies/ont.owl#strokeMapping">
        <rdf:type rdf:resource="https://www.AHDB/connected#Mapping"/>
        <implementation rdf:resource="http://www.co-ode.org/ontologies/ont.owl#strokeWebApi"/>
        <inputMapping rdf:resource="http://www.co-ode.org/ontologies/ont.owl#ageMapping"/>
        <inputMapping rdf:resource="http://www.co-ode.org/ontologies/ont.owl#avg_glucoseMapping"/>
        <inputMapping rdf:resource="http://www.co-ode.org/ontologies/ont.owl#heart_diseaseMapping"/>
        <inputMapping rdf:resource="http://www.co-ode.org/ontologies/ont.owl#hypertensionMapping"/>
        <interface rdf:resource="http://www.co-ode.org/ontologies/ont.owl#strokeModelInterface"/>
        <outputMapping rdf:resource="http://www.co-ode.org/ontologies/ont.owl#outMapping"/>
    </owl:NamedIndividual>
    


    <!-- http://www.co-ode.org/ontologies/ont.owl#strokeModel -->

    <owl:NamedIndividual rdf:about="http://www.co-ode.org/ontologies/ont.owl#strokeModel">
        <rdf:type rdf:resource="https://www.AHDB/connected#Model"/>
        <hasInterface rdf:resource="http://www.co-ode.org/ontologies/ont.owl#strokeModelInterface"/>
        <hasMaintainer rdf:resource="http://www.co-ode.org/ontologies/ont.owl#maintainer"/>
    </owl:NamedIndividual>
    


    <!-- http://www.co-ode.org/ontologies/ont.owl#strokeModelInterface -->

    <owl:NamedIndividual rdf:about="http://www.co-ode.org/ontologies/ont.owl#strokeModelInterface">
        <rdf:type rdf:resource="https://www.AHDB/connected#Interface"/>
        <expects rdf:resource="http://www.co-ode.org/ontologies/ont.owl#age"/>
        <expects rdf:resource="http://www.co-ode.org/ontologies/ont.owl#avg_glucose"/>
        <expects rdf:resource="http://www.co-ode.org/ontologies/ont.owl#heart_disease"/>
        <expects rdf:resource="http://www.co-ode.org/ontologies/ont.owl#hypertension"/>
        <returns rdf:resource="http://www.co-ode.org/ontologies/ont.owl#output"/>
    </owl:NamedIndividual>
    


    <!-- http://www.co-ode.org/ontologies/ont.owl#strokeWebApi -->

    <owl:NamedIndividual rdf:about="http://www.co-ode.org/ontologies/ont.owl#strokeWebApi">
        <rdf:type rdf:resource="https://www.AHDB/connected#WebAPI"/>
        <contentType>application/json</contentType>
        <entrypoint rdf:datatype="http://www.w3.org/2001/XMLSchema#anyURI">http://stroke-web-service:5000</entrypoint>
        <method rdf:datatype="http://www.w3.org/2001/XMLSchema#anyURI">post</method>
    </owl:NamedIndividual>
    


    <!-- http://www.co-ode.org/ontologies/ont.owl#user -->

    <owl:NamedIndividual rdf:about="http://www.co-ode.org/ontologies/ont.owl#user">
        <rdf:type rdf:resource="http://www.w3.org/2000/10/swap/pim/contact#Person"/>
        <foaf:familyName>Rossi</foaf:familyName>
        <foaf:givenName>Mario</foaf:givenName>
        <foaf:name>Mario Rossi</foaf:name>
        <foaf:homepage>http://example.org/mario</foaf:homepage>
        <foaf:mbox>mario.rossi@x-company.com</foaf:mbox>
    </owl:NamedIndividual>
    


    <!-- https://loinc.org/LA32903-9 -->

    <owl:NamedIndividual rdf:about="https://loinc.org/LA32903-9"/>
    


    <!-- https://loinc.org/15074-8 -->

    <owl:NamedIndividual rdf:about="https://loinc.org/15074-8"/>
    <rdf:Description>
        <rdfs:label>Christian D&apos;Errico</rdfs:label>
        <foaf:mbox>christian.derrico2@unibo.it</foaf:mbox>
    </rdf:Description>
    <rdf:Description>
        <rdfs:label>Christian D&apos;Errico</rdfs:label>
        <foaf:mbox>christian.derrico2@unibo.it</foaf:mbox>
    </rdf:Description>
    <rdf:Description>
        <rdfs:label>Christian D&apos;Errico</rdfs:label>
        <foaf:mbox>christian.derrico2@unibo.it</foaf:mbox>
    </rdf:Description>
    <rdf:Description>
        <rdfs:label>Christian D&apos;Errico</rdfs:label>
        <foaf:mbox>christian.derrico2@unibo.it</foaf:mbox>
    </rdf:Description>
    <rdf:Description>
        <rdfs:label>Christian D&apos;Errico</rdfs:label>
        <foaf:mbox>christian.derrico2@unibo.it</foaf:mbox>
    </rdf:Description>
</rdf:RDF>



<!-- Generated by the OWL API (version 4.5.29.2024-05-13T12:11:03Z) https://github.com/owlcs/owlapi -->

